core/mem_lemmas.v
@@ -11,6 +11,14 @@ Require Import Globalenvs.
 
 Require Import Extensionality.
 
+Lemma valid_block_dec: forall m b, {Mem.valid_block m b} +  {~Mem.valid_block m b}.
+Proof. intros.
+unfold Mem.valid_block.
+remember (plt b (Mem.nextblock m)).
+destruct s. left; assumption.
+right. intros N. xomega.
+Qed.
+
 Lemma Forall2_length {A B} {f:A -> B -> Prop} {l1 l2} (F:Forall2 f l1 l2): length l1 = length l2.
 Proof. induction F; trivial. simpl; rewrite IHF. trivial. Qed.
 
@@ -178,35 +186,91 @@ Proof. intros.
 Qed.
 
 (* A minimal preservation property we sometimes require. *)
+(*
+Definition readonly {F V} (ge: Genv.t F V) m1 b m2 :=
+    forall gv, Genv.find_var_info ge b = Some gv ->
+       gvar_readonly gv && negb (gvar_volatile gv) = true ->
+    forall ch ofs, Mem.load ch m2 b ofs = Mem.load ch m1 b ofs.
+*)
+
+Definition readonlyLD m1 b m2 :=
+    forall chunk ofs
+    (NWR: forall ofs', ofs <= ofs' < ofs + size_chunk chunk ->
+                          ~(Mem.perm m1 b ofs' Max Writable)),
+     Mem.load chunk m2 b ofs = Mem.load chunk m1 b ofs /\
+     (forall ofs', ofs <= ofs' < ofs + size_chunk chunk -> 
+        (forall k p, Mem.perm m1 b ofs' k p <-> Mem.perm m2 b ofs' k p)).
 
 Definition readonly m1 b m2 :=
-    (forall ofs : Z, ~ Mem.perm m1 b ofs Max Writable) ->
-    forall ch ofs, Mem.load ch m2 b ofs = Mem.load ch m1 b ofs.
+    forall n ofs
+    (NWR: forall i, 0 <= i < n ->
+                          ~(Mem.perm m1 b (ofs + i) Max Writable)),
+     Mem.loadbytes m2 b ofs n = Mem.loadbytes m1 b ofs n /\
+     (forall i, 0 <= i < n -> 
+        (forall k p, Mem.perm m1 b (ofs+i) k p <-> Mem.perm m2 b (ofs+i) k p)).
 
-Definition readonly_refl m b: readonly m b m.
-  Proof. red; intros. trivial. Qed. 
+Lemma readonly_readonlyLD m1 b m2: readonly m1 b m2 -> readonlyLD m1 b m2.
+Proof.
+  red; intros. destruct (H (size_chunk chunk) ofs); clear H.
+    intros. apply NWR. omega.
+  split; intros.
+    remember (Mem.load chunk m2 b ofs) as d; symmetry in Heqd; symmetry.
+    destruct d.
+    { destruct (Mem.load_loadbytes _ _ _ _ _ Heqd) as [bytes [LDB V]]; subst v.
+      apply Mem.load_valid_access in Heqd; destruct Heqd.
+      rewrite H0 in LDB. apply Mem.loadbytes_load; trivial.
+    }
+    { remember (Mem.load chunk m1 b ofs) as q; symmetry in Heqq; symmetry. 
+      destruct q; trivial.
+      destruct (Mem.load_loadbytes _ _ _ _ _ Heqq) as [bytes [LDB V]]; subst v.
+      apply Mem.load_valid_access in Heqq; destruct Heqq.
+      rewrite <- Heqd.
+      rewrite <- H0 in LDB. apply Mem.loadbytes_load; trivial. }
+  specialize (H1 (ofs'-ofs)). rewrite Zplus_minus in H1. apply H1. omega.
+Qed.
+
+Lemma readonly_refl m b: readonly m b m.
+  Proof. red; intuition. Qed.
+
+Lemma readonlyLD_refl m b: readonlyLD m b m.
+  Proof. red; intuition. Qed.
+
+Lemma readonlyLD_trans m1 m2 m3 b: readonlyLD m1 b m2 -> readonlyLD m2 b m3 -> readonlyLD m1 b m3.
+  Proof. red; intros. destruct (H _ _ NWR); clear H. 
+    destruct (H0 chunk ofs); clear H0.
+      intros. intros N. apply (NWR _ H). apply (H2 _ H). assumption.
+    split. rewrite <- H1. assumption.
+    intros. destruct (H2 _ H0 k p); clear H2. destruct (H3 _ H0 k p); clear H3. 
+      split; eauto. 
+  Qed.
+
+Lemma readonly_trans m1 m2 m3 b: readonly m1 b m2 -> readonly m2 b m3 -> readonly m1 b m3.
+  Proof. red; intros. destruct (H _ _ NWR); clear H. 
+    destruct (H0 n ofs); clear H0.
+      intros. intros N. apply (NWR _ H). apply (H2 _ H). assumption.
+    split. rewrite <- H1. assumption.
+    intros. destruct (H2 _ H0 k p); clear H2. destruct (H3 _ H0 k p); clear H3. 
+      split; eauto. 
+  Qed.
 
 Definition mem_forward (m1 m2:mem) :=
   forall b, Mem.valid_block m1 b ->
     (Mem.valid_block m2 b 
      /\ (forall ofs p, Mem.perm m2 b ofs Max p -> Mem.perm m1 b ofs Max p)
-     /\ readonly m1 b m2).
+     (*/\ readonly m1 b m2*)).
 
 Lemma mem_forward_refl: forall m, mem_forward m m.
 Proof. intros m b H. split; trivial.
-  split; eauto. apply readonly_refl.
+(*  split; eauto. apply readonly_refl.*)
 Qed. 
 
 Lemma mem_forward_trans: forall m1 m2 m3, 
   mem_forward m1 m2 -> mem_forward m2 m3 -> mem_forward m1 m3.
 Proof. intros. intros  b Hb.
-  destruct (H _ Hb) as [? [? ?]]. 
-  destruct (H0 _ H1) as [? [? ?]].
+  destruct (H _ Hb) as [? ?]. 
+  destruct (H0 _ H1) as [? ?].
   split; eauto.
-  split; eauto.
-  red; intros. rewrite H6. apply H3. trivial.
-   intros z N. apply H2 in N. apply (H7 _ N).
-Qed. 
+Qed.
 
 Lemma forward_unchanged_trans: forall P m1 m2 m3,
 Mem.unchanged_on P m1 m2 -> Mem.unchanged_on P m2 m3 ->
@@ -517,7 +581,7 @@ Lemma fwd_maxpermorder: forall m1 m2 (FWD: mem_forward m1 m2) (b:block)
   Mem.perm_order'' (PMap.get b (Mem.mem_access m1) ofs Max)
                    (PMap.get b (Mem.mem_access m2) ofs Max).
 Proof.
-  intros. destruct (FWD b) as [? [? RD]]; try assumption. 
+  intros. destruct (FWD b) as [? ?]; try assumption. 
   remember ((PMap.get b (Mem.mem_access m2) ofs Max)) as z.
   destruct z; apply eq_sym in Heqz; simpl  in *.
   remember ((PMap.get b (Mem.mem_access m1) ofs Max)) as zz.
@@ -642,25 +706,7 @@ Proof. intros.
 Qed.
 
 (******** Compatibility of memory operation with [mem_forward] ********)
-
-Lemma store_forward: forall m b ofs v ch m'
-      (M:Mem.store ch m b ofs v = Some m'),
-      mem_forward m m'.
-Proof. intros.
-  split; intros.
-    eapply Mem.store_valid_block_1; eassumption.
-  split; intros.
-    eapply Mem.perm_store_2; eassumption.
-  red; intros. 
-    eapply Mem.load_store_other; try eassumption.
-    destruct (eq_block b0 b); subst. 2: left; trivial.
-    elim (H0 ofs).
-    eapply Mem.perm_max. 
-    eapply Mem.store_valid_access_3; try eassumption.
-    specialize (size_chunk_pos ch); intros; omega.
-Qed.
-
-Lemma storebytes_nil m b ofs m': Mem.storebytes m b ofs nil = Some m' -> 
+Lemma load_storebytes_nil m b ofs m': Mem.storebytes m b ofs nil = Some m' -> 
   forall ch bb z, Mem.load ch m' bb z = Mem.load ch m bb z.
 Proof. intros.
   remember (Mem.load ch m' bb z) as u'; symmetry in Hequ'; destruct u'.
@@ -690,6 +736,128 @@ Proof. intros.
     intros; simpl; trivial.
 Qed.
 
+Lemma loadbytes_storebytes_nil m b ofs m': Mem.storebytes m b ofs nil = Some m' -> 
+  forall n bb z, Mem.loadbytes m' bb z n = Mem.loadbytes m bb z n.
+Proof. intros.
+  remember (Mem.loadbytes m' bb z n) as u'; symmetry in Hequ'; destruct u'.
+      symmetry.
+      eapply Mem.loadbytes_unchanged_on; try eassumption.
+      instantiate (1:= fun b ofs => True).
+      split; intros.
+        split; intros.
+          eapply Mem.perm_storebytes_2; eassumption.
+          eapply Mem.perm_storebytes_1; eassumption.
+      rewrite (Mem.storebytes_mem_contents _ _ _ _ _ H).
+      destruct (eq_block b0 b); subst. rewrite PMap.gss; trivial.
+      rewrite PMap.gso; trivial.
+    intros; simpl; trivial.
+
+    remember (Mem.loadbytes m bb z n) as u; symmetry in Hequ; destruct u; trivial. 
+      rewrite <- Hequ'; clear Hequ'.
+      eapply Mem.loadbytes_unchanged_on; try eassumption.
+      instantiate (1:= fun b ofs => True).
+      split; intros.
+        split; intros.
+          eapply Mem.perm_storebytes_1; eassumption.
+          eapply Mem.perm_storebytes_2; eassumption.
+      rewrite (Mem.storebytes_mem_contents _ _ _ _ _ H). 
+      destruct (eq_block b0 b); subst. rewrite PMap.gss; trivial.
+      rewrite PMap.gso; trivial.
+    intros; simpl; trivial.
+Qed.
+
+Lemma storebytes_forward: forall m b ofs bytes m'
+      (M: Mem.storebytes m b ofs bytes = Some m'),
+      mem_forward m m'.
+Proof. intros.
+  split; intros.
+    eapply Mem.storebytes_valid_block_1; eassumption.
+    eapply Mem.perm_storebytes_2; eassumption.
+Qed.
+
+Lemma storebytes_readonlyLD: forall m b ofs bytes m'
+      (M: Mem.storebytes m b ofs bytes = Some m'),
+      forall b, Mem.valid_block m b -> readonlyLD m b m'.
+Proof.
+  red; intros.
+  split. 
+    destruct bytes.
+      eapply load_storebytes_nil; eassumption.
+    eapply Mem.load_storebytes_other; try eassumption.
+    destruct (eq_block b0 b); subst. 2: left; trivial. right.
+    apply Mem.storebytes_range_perm in M.
+    destruct (zle (ofs0 + size_chunk chunk) ofs). left; trivial. right.
+    destruct (zle (ofs + Z.of_nat (length (m0 :: bytes)))  ofs0); trivial.
+    exfalso.
+    destruct (zle ofs0 ofs).
+      apply (NWR ofs). omega.
+                      eapply Mem.perm_max. apply M. simpl. specialize (Zle_0_nat (length bytes)); intros; xomega.
+      elim (NWR ofs0). specialize (size_chunk_pos chunk); intros; omega.
+                      eapply Mem.perm_max. apply M. omega.
+  split; intros. eapply Mem.perm_storebytes_1; eassumption. eapply Mem.perm_storebytes_2; eassumption.
+Qed.
+
+Lemma storebytes_readonly: forall m b ofs bytes m'
+      (M: Mem.storebytes m b ofs bytes = Some m'),
+      forall b, Mem.valid_block m b -> readonly m b m'.
+Proof.
+  red; intros.
+  destruct (zle n 0).
+  { split; intros. repeat rewrite Mem.loadbytes_empty; trivial. omega. }
+  split. 
+    destruct bytes.
+      eapply loadbytes_storebytes_nil; eassumption.
+    eapply Mem.loadbytes_storebytes_other; try eassumption. omega.
+    destruct (eq_block b0 b); subst. 2: left; trivial. right.
+    apply Mem.storebytes_range_perm in M.
+    destruct (zle (ofs0 + n) ofs). left; trivial. right.
+    destruct (zle (ofs + Z.of_nat (length (m0 :: bytes)))  ofs0); trivial.
+    exfalso. remember (Z.of_nat (length (m0 :: bytes))) as l. assert (0 < l). simpl in Heql. xomega. clear Heql. 
+    destruct (zle ofs0 ofs).
+      apply (NWR (ofs-ofs0)). omega.
+                  eapply Mem.perm_max. apply M. rewrite Zplus_minus. omega.
+      elim (NWR 0). omega.
+                    eapply Mem.perm_max. apply M. omega.
+  split; intros. eapply Mem.perm_storebytes_1; eassumption. eapply Mem.perm_storebytes_2; eassumption.
+Qed.
+
+Lemma store_forward: forall m b ofs v ch m'
+      (M:Mem.store ch m b ofs v = Some m'),
+      mem_forward m m'.
+Proof. intros.
+  apply Mem.store_storebytes in M.
+  eapply storebytes_forward; eassumption.
+Qed.
+    
+Lemma store_readonly: forall m b ofs v ch m'
+      (M:Mem.store ch m b ofs v = Some m'),
+      forall b, Mem.valid_block m b -> readonly m b m'.
+Proof. intros.
+  apply Mem.store_storebytes in M.
+  eapply storebytes_readonly; eassumption.
+Qed.
+    
+     
+
+
+(*
+Lemma store_forward: forall m b ofs v ch m'
+      (M:Mem.store ch m b ofs v = Some m'),
+      mem_forward m m'.
+Proof. intros.
+  split; intros.
+    eapply Mem.store_valid_block_1; eassumption.
+  split; intros.
+    eapply Mem.perm_store_2; eassumption.
+  red; intros. 
+    eapply Mem.load_store_other; try eassumption.
+    destruct (eq_block b0 b); subst. 2: left; trivial.
+    elim (H0 ofs).
+    eapply Mem.perm_max. 
+    eapply Mem.store_valid_access_3; try eassumption.
+    specialize (size_chunk_pos ch); intros; omega.
+Qed.
+
 Lemma storebytes_forward: forall m b ofs bytes m'
       (M: Mem.storebytes m b ofs bytes = Some m'),
       mem_forward m m'.
@@ -706,6 +874,7 @@ Proof. intros.
     apply Mem.storebytes_range_perm in M.
     elim (H0 ofs). eapply Mem.perm_max. eapply M. simpl; xomega.
 Qed.
+*)
 
 Lemma alloc_forward: 
       forall m lo hi m' b
@@ -714,12 +883,69 @@ Lemma alloc_forward:
 Proof. intros.
 split; intros.
   eapply Mem.valid_block_alloc; eassumption.
-split; intros.
   eapply Mem.perm_alloc_4; try eassumption.
   intros N; subst. eapply (Mem.fresh_block_alloc _ _ _ _ _ A H).
-red; intros. eapply Mem.load_alloc_unchanged; try eassumption.
 Qed.
 
+Lemma unchanged_on_sym P m m' b:
+  Mem.unchanged_on P m m' -> Mem.valid_block m b ->
+  Mem.unchanged_on (fun bb z => P bb z /\ bb=b) m' m.
+Proof. intros.
+  destruct H as [U1 U2].
+  split; intros; destruct H; subst b0.
+    split; intros; eapply U1; trivial.
+    rewrite U2; trivial. eapply U1; trivial.
+Qed.
+    
+Lemma loadbytes_unchanged_on (P : block -> Z -> Prop) m m' b ofs n:
+  Mem.unchanged_on P m m' -> Mem.valid_block m b ->
+  (forall i : Z, ofs <= i < ofs + n -> P b i) ->
+  Mem.loadbytes m b ofs n = Mem.loadbytes m' b ofs n.
+Proof. intros.
+  remember (Mem.loadbytes m b ofs n) as d; symmetry in Heqd.
+  destruct d. symmetry. eapply Mem.loadbytes_unchanged_on; eassumption.
+  remember (Mem.loadbytes m' b ofs n) as q; symmetry in Heqq.
+  destruct q; trivial.
+  erewrite Mem.loadbytes_unchanged_on in Heqd; try eapply Heqq. discriminate.
+    eapply unchanged_on_sym; eassumption.
+    simpl; intros. split; auto.
+Qed.
+
+Lemma loadbytes_alloc_unchanged m1 lo hi m2 b :
+  Mem.alloc m1 lo hi = (m2, b) ->
+  forall n (b' : block) (ofs : Z),
+  Mem.valid_block m1 b' ->
+  Mem.loadbytes m2 b' ofs n = Mem.loadbytes m1 b' ofs n.
+Proof. intros. symmetry.
+  eapply loadbytes_unchanged_on; try eassumption.
+  eapply (Mem.alloc_unchanged_on (fun bb z => True)). eassumption.
+  simpl. trivial.
+Qed.
+
+Lemma alloc_readonly: 
+      forall m lo hi m' b
+      (A: Mem.alloc m lo hi = (m',b)),
+      forall b, Mem.valid_block m b -> readonly m b m'.
+Proof. red; intros.
+  split. eapply loadbytes_alloc_unchanged; try eassumption.
+  intros; split. eapply Mem.perm_alloc_1; eassumption. 
+     intros. eapply Mem.perm_alloc_4; try eassumption.
+     apply Mem.fresh_block_alloc in A. 
+     destruct (eq_block b0 b); trivial. subst. elim (A H).
+Qed.
+
+Lemma alloc_readonlyLD: 
+      forall m lo hi m' b
+      (A: Mem.alloc m lo hi = (m',b)),
+      forall b, Mem.valid_block m b -> readonlyLD m b m'.
+Proof. red; intros.
+  split. eapply Mem.load_alloc_unchanged; try eassumption.
+  intros; split. eapply Mem.perm_alloc_1; eassumption. 
+     intros. eapply Mem.perm_alloc_4; try eassumption.
+     apply Mem.fresh_block_alloc in A. 
+     destruct (eq_block b0 b); trivial. subst. elim (A H).
+Qed.
+(*
 Lemma free_forward: forall b z0 z m m'
       (M: Mem.free m b z0 z = Some m'),
       mem_forward m m'.
@@ -739,6 +965,102 @@ red; intros. eapply Mem.load_free; try eassumption.
     constructor.
   right; left; trivial.
 Qed.
+*)
+Lemma free_forward: forall b z0 z m m'
+      (M: Mem.free m b z0 z = Some m'),
+      mem_forward m m'.
+Proof. intros.
+split; intros.
+  eapply Mem.valid_block_free_1; eassumption. 
+  eapply Mem.perm_free_3; eassumption.
+Qed.
+
+Lemma loadbytes_free m1 bf lo hi m2:
+  Mem.free m1 bf lo hi = Some m2 ->
+  forall n (b : block) (ofs : Z),
+  b <> bf \/ lo >= hi \/ ofs + n <= lo \/ hi <= ofs ->
+  Mem.loadbytes m2 b ofs n = Mem.loadbytes m1 b ofs n.
+Proof. intros.
+  remember (Mem.loadbytes m2 b ofs n) as d; symmetry in Heqd.
+  destruct d.
+  { apply loadbytes_D in Heqd; destruct Heqd. 
+    rewrite (Mem.free_result _ _ _ _ _ H) in H2. simpl in H2.
+    assert (F: Mem.range_perm m1 b ofs (ofs + n) Cur Readable).
+      red; intros. eapply Mem.perm_free_3. eassumption.
+        eapply H1. assumption.
+    apply Mem.range_perm_loadbytes in F. destruct F as [bytes F]; rewrite F.
+    apply loadbytes_D in F. destruct F. rewrite <- H2 in H4. subst; trivial.
+  }
+  { remember (Mem.loadbytes m1 b ofs n) as q; symmetry in Heqq.
+    destruct q; trivial.
+    apply loadbytes_D in Heqq. destruct Heqq as [F C].
+    assert (Mem.range_perm m2 b ofs (ofs + n) Cur Readable).
+    { red; intros. eapply Mem.perm_free_1. eassumption.
+        destruct H0. left; trivial. right. omega.
+      apply F. trivial.
+    }
+    apply Mem.range_perm_loadbytes in H1. rewrite Heqd in H1. destruct H1; discriminate.
+  }
+Qed. 
+
+Lemma free_readonlyLD: forall b lo hi m m'
+      (M: Mem.free m b lo hi = Some m'),
+      forall b, Mem.valid_block m b -> readonlyLD m b m'.
+Proof. red; intros. 
+split. 
+  eapply Mem.load_free; try eassumption.
+  destruct (eq_block b0 b); try subst b0. 2: left; trivial.
+  right; destruct (zle hi lo). left; omega. right.
+  destruct (zle (ofs + size_chunk chunk) lo). left; trivial. right.
+  destruct (zle hi ofs); trivial. exfalso.
+  destruct (zle ofs lo).
+    eapply (NWR lo); clear NWR. omega.
+    eapply Mem.perm_max.
+    eapply Mem.perm_implies. 
+      eapply Mem.free_range_perm; try eassumption. omega. constructor.
+  eapply (NWR ofs); clear NWR. specialize (size_chunk_pos chunk). intros; omega.
+    eapply Mem.perm_max.
+    eapply Mem.perm_implies. 
+      eapply Mem.free_range_perm; try eassumption. omega. constructor.
+intros. specialize (Mem.free_range_perm _ _ _ _ _ M); intros F. red in F.
+    split; intros. eapply Mem.perm_free_1; try eassumption.
+      destruct (eq_block b0 b); try subst b0. 2: left; trivial. right. 
+      destruct (zlt ofs' lo). left; trivial. right. destruct (zle hi ofs'). trivial.
+      elim (NWR _ H0). (* specialize (size_chunk_pos chunk). intros; omega.*)
+      eapply Mem.perm_max. eapply Mem.perm_implies. apply F. omega. constructor.
+    eapply Mem.perm_free_3; try eassumption.
+Qed.
+
+Lemma free_readonly: forall b lo hi m m'
+      (M: Mem.free m b lo hi = Some m'),
+      forall b, Mem.valid_block m b -> readonly m b m'.
+Proof. red; intros.
+destruct (zle n 0).
+  split. repeat rewrite Mem.loadbytes_empty; trivial.
+         intros; omega.
+split. 
+  eapply loadbytes_free; try eassumption.
+  destruct (eq_block b0 b); try subst b0. 2: left; trivial.
+  right; destruct (zle hi lo). left; omega. right.
+  destruct (zle (ofs + n) lo). left; trivial. right.
+  destruct (zle hi ofs); trivial. exfalso.
+  destruct (zle lo ofs).
+    eapply (NWR 0); clear NWR. omega.
+    eapply Mem.perm_max.
+    eapply Mem.perm_implies. 
+      eapply Mem.free_range_perm; try eassumption. omega. constructor.
+  eapply (NWR (lo - ofs)); clear NWR. omega. rewrite Zplus_minus.
+    eapply Mem.perm_max.
+    eapply Mem.perm_implies. 
+      eapply Mem.free_range_perm; try eassumption. omega. constructor.
+intros. specialize (Mem.free_range_perm _ _ _ _ _ M); intros F. red in F.
+    split; intros. eapply Mem.perm_free_1; try eassumption.
+      destruct (eq_block b0 b); try subst b0. 2: left; trivial. right. 
+      destruct (zlt (ofs + i) lo). left; trivial. right. destruct (zle hi (ofs+i)). trivial.
+      elim (NWR _ H0). (* specialize (size_chunk_pos chunk). intros; omega.*)
+      eapply Mem.perm_max. eapply Mem.perm_implies. apply F. omega. constructor.
+    eapply Mem.perm_free_3; try eassumption.
+Qed.
 
 Lemma freelist_forward: forall l m m'
       (M: Mem.free_list m l = Some m'),
@@ -752,6 +1074,36 @@ Proof. intros l.
   specialize (IHl _ _ H0).
   apply free_forward in Heqd.
   eapply mem_forward_trans; eassumption. 
+Qed.
+
+Lemma freelist_readonly: forall l m m'
+      (M: Mem.free_list m l = Some m'), 
+      forall b, Mem.valid_block m b -> readonly m b m'.
+Proof.
+  induction l; simpl; intros.
+    inv M. apply readonly_refl.
+  destruct a. destruct p.
+  remember (Mem.free m b0 z0 z) as d.
+  destruct d; inv M; apply eq_sym in Heqd.
+  specialize (IHl _ _ H1).
+  eapply readonly_trans. 
+    eapply (free_readonly _ _ _ _ _ Heqd _ H).
+  eapply IHl. eapply free_forward; eassumption.
+Qed.
+
+Lemma freelist_readonlyLD: forall l m m'
+      (M: Mem.free_list m l = Some m'), 
+      forall b, Mem.valid_block m b -> readonlyLD m b m'.
+Proof.
+  induction l; simpl; intros.
+    inv M. apply readonlyLD_refl.
+  destruct a. destruct p.
+  remember (Mem.free m b0 z0 z) as d.
+  destruct d; inv M; apply eq_sym in Heqd.
+  specialize (IHl _ _ H1).
+  eapply readonlyLD_trans. 
+    eapply (free_readonlyLD _ _ _ _ _ Heqd _ H).
+  eapply IHl. eapply free_forward; eassumption.
 Qed.
 
 Lemma forward_nextblock: forall m m',
@@ -856,14 +1208,6 @@ forall ch m addr v m',
 Mem.storev ch m addr v = Some m' -> 
 (forall b, Mem.valid_block m' b -> Mem.valid_block m b).
 Proof. intros. destruct addr; inv H. eapply Mem.store_valid_block_2; eauto. Qed.
-
-Lemma valid_block_dec: forall m b, {Mem.valid_block m b} +  {~Mem.valid_block m b}.
-Proof. intros.
-unfold Mem.valid_block.
-remember (plt b (Mem.nextblock m)).
-destruct s. left; assumption.
-right. intros N. xomega.
-Qed.
 
 (*This is an [F,V]-independent definition of meminj_preserves_globals*)
 Definition meminj_preserves_globals_ind (globals: (block->Prop)*(block->Prop)) f :=
@@ -1078,19 +1422,18 @@ Proof. intros.
 Qed.
 
 Lemma forward_unchanged_on: forall m m' (FWD: mem_forward m m')
-           b ofs (P: ~ Mem.perm m b ofs Max Nonempty),
+           b ofs (NP: ~ Mem.perm m b ofs Max Nonempty),
      Mem.unchanged_on (fun b' ofs' => b' = b /\ ofs' = ofs) m m'.
 Proof. intros.
 split; intros. 
   destruct H; subst. 
-  split; intros; elim P. 
-    eapply Mem.perm_max. 
-    eapply Mem.perm_implies; try eassumption. apply perm_any_N. 
-    eapply FWD. assumption. 
+  split; intros; elim NP. 
     eapply Mem.perm_max. 
     eapply Mem.perm_implies; try eassumption. apply perm_any_N.
+    destruct (FWD _ H0) as [VB' P]. eapply Mem.perm_implies. 
+       apply P. eapply Mem.perm_max; eassumption. apply perm_any_N.
 destruct H; subst. 
-  elim P. eapply Mem.perm_max. 
+  elim NP. eapply Mem.perm_max. 
   eapply Mem.perm_implies; try eassumption. apply perm_any_N.
 Qed.
 
@@ -1137,14 +1480,14 @@ Lemma unchanged_on_perm_intersection: forall m m' U (Fwd: mem_forward m m'),
     split; intros Hyp.
     split; intros; eapply Hyp; eauto. apply H. apply H.
     split; intros.
-      remember (Mem.perm_dec m b ofs Max Nonempty).
+    remember (Mem.perm_dec m b ofs Max Nonempty).
       destruct s; clear Heqs.
          eapply Hyp; eauto.
       split; intros. exfalso. apply n; clear Hyp n.
          eapply Mem.perm_implies. eapply Mem.perm_max; eassumption. 
                apply perm_any_N.
         exfalso. apply n; clear Hyp n.
-         eapply (Fwd _ H0).
+        destruct (Fwd _ H0) as [VB' P]. apply P.
            eapply Mem.perm_implies. eapply Mem.perm_max; eassumption. 
                apply perm_any_N.
      eapply Hyp; trivial.
@@ -1170,6 +1513,17 @@ destruct U1 as [P1 V1]; destruct U2 as [P2 V2].
   apply P1; trivial. eapply Mem.perm_valid_block; eassumption.
 Qed.
 
+Axiom ec_readonly_perm:
+  forall (ef : external_function) (F V : Type) (ge : Genv.t F V)
+    (vargs : list val) (m1 : mem) (t : trace) (vres : val) (m2 : mem)
+    (chunk : memory_chunk) (b : block) (ofs : Z),
+  external_call ef ge vargs m1 t vres m2 ->
+  Mem.valid_block m1 b ->
+  (forall ofs' : Z,
+   ofs <= ofs' < ofs + size_chunk chunk -> ~ Mem.perm m1 b ofs' Max Writable) ->
+  forall ofs', ofs <= ofs' < ofs + size_chunk chunk ->
+    forall k p, Mem.perm m1 b ofs' k p <-> Mem.perm m2 b ofs' k p.
+
 Lemma external_call_mem_forward:
   forall (ef : external_function) (F V : Type) (ge : Genv.t F V)
     (vargs : list val) (m1 : mem) (t : trace) (vres : val) (m2 : mem),
@@ -1177,9 +1531,24 @@ Lemma external_call_mem_forward:
 Proof.
 intros. intros b Hb.
 split; intros. eapply external_call_valid_block; eauto.
-split. intros. eapply external_call_max_perm; eauto.
-red; intros. eapply ec_readonly. apply (external_call_spec ef). eassumption. eassumption.
-  intros. apply H0.
+eapply external_call_max_perm; eauto.
+Qed.
+
+Axiom external_call_readonly:
+  forall (ef : external_function) (F V : Type) (ge : Genv.t F V)
+    (vargs : list val) (m1 : mem) (t : trace) (vres : val) (m2 : mem),
+    external_call ef ge vargs m1 t vres m2 -> 
+  forall b, Mem.valid_block m1 b -> readonly m1 b m2. 
+
+Lemma external_call_readonlyLD:
+  forall (ef : external_function) (F V : Type) (ge : Genv.t F V)
+    (vargs : list val) (m1 : mem) (t : trace) (vres : val) (m2 : mem),
+    external_call ef ge vargs m1 t vres m2 -> 
+  forall b, Mem.valid_block m1 b -> readonlyLD m1 b m2. 
+Proof. red; intros.
+  split. eapply ec_readonly; trivial.
+         apply (external_call_spec ef). eassumption.
+  eapply ec_readonly_perm; eassumption.
 Qed.
 
 Definition val_has_type_opt' (v: option val) (ty: typ) :=
